simplify creation of ranges

src/Init/Data/Range/Polymorphic/Instances.lean
@@ -6,12 +6,14 @@ Authors: Paul Reichert
 module
 
 prelude
-public import Init.Data.Range.Polymorphic.Basic
 public import Init.Data.Order.Classes
-
-open Std PRange
+public import Init.Data.Range.Polymorphic.Basic
+import Init.Data.Nat.Lemmas
+import Init.Data.Order.Lemmas
 
 public section
+
+namespace Std.PRange
 
 instance [LE α] [LT α] [UpwardEnumerable α] [LawfulUpwardEnumerable α]
     [LawfulUpwardEnumerableLE α] [LawfulOrderLT α] : LawfulUpwardEnumerableLT α where
@@ -94,3 +96,73 @@ instance [LE α] [Total (α := α) (· ≤ ·)] [UpwardEnumerable α] [LawfulUpw
 
 instance [UpwardEnumerable α] : LawfulUpwardEnumerableUpperBound .unbounded α where
   isSatisfied_of_le _ _ _ _ _ := .intro
+
+@[inline]
+abbrev RangeSize.openOfClosed [RangeSize .closed α] : RangeSize .open α where
+  size bound a := RangeSize.size (shape := .closed) bound a - 1
+
+attribute [local instance] RangeSize.openOfClosed in
+instance LawfulRangeSize.open_of_closed [UpwardEnumerable α] [LE α] [DecidableLE α]
+    [LT α] [DecidableLT α] [LawfulOrderLT α] [IsPartialOrder α]
+    [LawfulUpwardEnumerable α] [LawfulUpwardEnumerableLE α]
+    [RangeSize .closed α] [LawfulRangeSize .closed α] :
+    LawfulRangeSize .open α where
+  size_eq_zero_of_not_isSatisfied bound a h := by
+    simp [SupportsUpperBound.IsSatisfied] at h
+    simp [RangeSize.size]
+    by_cases h' : a ≤ bound
+    · match hs : UpwardEnumerable.succ? a with
+      | none => rw [LawfulRangeSize.size_eq_one_of_succ?_eq_none (h := h') (h' := by omega)]
+      | some b =>
+        rw [LawfulRangeSize.size_eq_succ_of_succ?_eq_some (h := h') (h' := hs)]
+        have : ¬ b ≤ bound := by
+          intro hb
+          have : a < b := by
+            rw [LawfulUpwardEnumerableLT.lt_iff]
+            exact ⟨0, by simpa [UpwardEnumerable.succMany?_one] using hs⟩
+          exact h (lt_of_lt_of_le this hb)
+        rw [LawfulRangeSize.size_eq_zero_of_not_isSatisfied (h := this)]
+    · suffices RangeSize.size (shape := .closed) bound a = 0 by omega
+      exact LawfulRangeSize.size_eq_zero_of_not_isSatisfied _ _ h'
+  size_eq_one_of_succ?_eq_none bound a h h' := by
+    exfalso
+    simp [SupportsUpperBound.IsSatisfied, LawfulUpwardEnumerableLT.lt_iff] at h
+    obtain ⟨n, hn⟩ := h
+    simp [LawfulUpwardEnumerable.succMany?_succ_eq_succ?_bind_succMany?, h'] at hn
+  size_eq_succ_of_succ?_eq_some bound a a' h h' := by
+    simp [SupportsUpperBound.IsSatisfied] at h
+    simp [RangeSize.size]
+    rw [LawfulRangeSize.size_eq_succ_of_succ?_eq_some (h := le_of_lt h) (h' := h')]
+    rw [← Nat.sub_add_comm]
+    · omega
+    · simp [Nat.succ_le_iff, LawfulRangeSize.size_pos_iff_isSatisfied,
+        SupportsUpperBound.IsSatisfied]
+      rw [LawfulUpwardEnumerableLE.le_iff]
+      rw [LawfulUpwardEnumerableLT.lt_iff] at h
+      refine ⟨h.choose, ?_⟩
+      simpa [LawfulUpwardEnumerable.succMany?_succ_eq_succ?_bind_succMany?, h'] using h.choose_spec
+
+instance LawfulRangeSize.instHasFiniteRanges [UpwardEnumerable α] [LawfulUpwardEnumerable α]
+    [RangeSize su α]
+    [SupportsUpperBound su α] [LawfulRangeSize su α] : HasFiniteRanges su α where
+  finite init bound := by
+    refine ⟨RangeSize.size bound init, ?_⟩
+    generalize hn : RangeSize.size bound init = n
+    induction n generalizing init with
+    | zero =>
+      simp only [LawfulRangeSize.size_eq_zero_iff_not_isSatisfied] at hn
+      simp [UpwardEnumerable.succMany?_zero, hn]
+    | succ =>
+      rename_i n ih
+      rw [LawfulUpwardEnumerable.succMany?_succ_eq_succ?_bind_succMany?]
+      match hs : UpwardEnumerable.succ? init with
+      | none => simp
+      | some a =>
+        simp only [Option.bind_some]
+        apply ih
+        have : SupportsUpperBound.IsSatisfied bound init :=
+          LawfulRangeSize.size_pos_iff_isSatisfied.mp (by omega)
+        rw [LawfulRangeSize.size_eq_succ_of_succ?_eq_some (h := this) (h' := hs)] at hn
+        omega
+
+end Std.PRange
